Matroid/Minor/Rank.lean
@@ -8,26 +8,26 @@ variable {α : Type*} {M N : Matroid α} {I J C D X Y Z : Set α} {e f : α}
 
 section Delete
 
-@[simp] theorem delete_er_eq' (M : Matroid α) (D X : Set α) : (M ＼ D).er X = M.er (X \ D) := by
+@[simp] lemma delete_er_eq' (M : Matroid α) (D X : Set α) : (M ＼ D).er X = M.er (X \ D) := by
   rw [← restrict_compl, restrict_er_eq', diff_eq, inter_comm M.E, ← inter_assoc, ← diff_eq,
     er_inter_ground_eq]
 
-theorem delete_er_eq (M : Matroid α) (h : Disjoint X D) : (M ＼ D).er X = M.er X := by
+lemma delete_er_eq (M : Matroid α) (h : Disjoint X D) : (M ＼ D).er X = M.er X := by
   rwa [delete_er_eq', sdiff_eq_left.2]
 
-theorem delete_er_eq_delete_er_diff (M : Matroid α) (D X : Set α) :
+lemma delete_er_eq_delete_er_diff (M : Matroid α) (D X : Set α) :
     (M ＼ D).er X = (M ＼ D).er (X \ D) := by
   simp
 
-@[simp] theorem delete_rFin_iff : (M ＼ D).rFin X ↔ M.rFin (X \ D) := by
+@[simp] lemma delete_rFin_iff : (M ＼ D).rFin X ↔ M.rFin (X \ D) := by
   rw [← er_lt_top_iff, delete_er_eq', er_lt_top_iff]
 
-theorem Coindep.delete_erk_eq (hX : M.Coindep X) : (M ＼ X).erk = M.erk := by
+lemma Coindep.delete_erk_eq (hX : M.Coindep X) : (M ＼ X).erk = M.erk := by
   rw [coindep_iff_cl_compl_eq_ground] at hX
   rw [erk_eq_er_ground, delete_ground, delete_er_eq', diff_diff, union_self, ← er_cl_eq, hX,
     erk_eq_er_ground]
 
-theorem Indep.delete_erk_dual_eq (hI : M.Indep I) : (M ／ I)✶.erk = M✶.erk := by
+lemma Indep.delete_erk_dual_eq (hI : M.Indep I) : (M ／ I)✶.erk = M✶.erk := by
   rw [← hI.coindep.delete_erk_eq, contract_dual_eq_dual_delete]
 
 end Delete
@@ -38,45 +38,45 @@ The definition suggests that `X` and `Y` should be disjoint, but it is also a na
 expression when `X ⊆ Y`, and sometimes more generally. -/
 noncomputable def relRank (M : Matroid α) (X Y : Set α) : ℕ∞ := (M ／ X).er Y
 
-theorem relRank_eq_er_contract (M : Matroid α) (X Y : Set α) : M.relRank X Y = (M ／ X).er Y := rfl
+lemma relRank_eq_er_contract (M : Matroid α) (X Y : Set α) : M.relRank X Y = (M ／ X).er Y := rfl
 
-theorem relRank_le_er (M : Matroid α) (X Y : Set α) : M.relRank X Y ≤ M.er Y := by
+lemma relRank_le_er (M : Matroid α) (X Y : Set α) : M.relRank X Y ≤ M.er Y := by
   obtain ⟨I, hI⟩ := (M ／ X).exists_basis (Y ∩ (M ／ X).E)
   rw [relRank, ← er_inter_ground_eq, ← hI.encard, ← hI.indep.of_contract.er]
   exact M.er_mono (hI.subset.trans (inter_subset_left _ _))
 
-theorem relRank_eq_er_diff_contract (M : Matroid α) (X Y : Set α) :
+lemma relRank_eq_er_diff_contract (M : Matroid α) (X Y : Set α) :
     M.relRank X Y = (M ／ X).er (Y \ X) := by
   rw [relRank_eq_er_contract, ← er_cl_eq, contract_cl_eq, eq_comm, ← er_cl_eq, contract_cl_eq,
     diff_union_self]
 
-theorem relRank_eq_diff_right (M : Matroid α) (X Y : Set α) : M.relRank X Y = M.relRank X (Y \ X) :=
+lemma relRank_eq_diff_right (M : Matroid α) (X Y : Set α) : M.relRank X Y = M.relRank X (Y \ X) :=
   M.relRank_eq_er_diff_contract X Y
 
-theorem relRank_mono_right (M : Matroid α) (X : Set α) {Y Y' : Set α} (hYY' : Y ⊆ Y') :
+lemma relRank_mono_right (M : Matroid α) (X : Set α) {Y Y' : Set α} (hYY' : Y ⊆ Y') :
     M.relRank X Y ≤ M.relRank X Y' :=
   (M ／ X).er_mono hYY'
 
-theorem relRank_mono_left (M : Matroid α) {X X' : Set α} (Y : Set α) (h : X ⊆ X') :
+lemma relRank_mono_left (M : Matroid α) {X X' : Set α} (Y : Set α) (h : X ⊆ X') :
     M.relRank X' Y ≤ M.relRank X Y := by
   rw [relRank, relRank, ← union_diff_cancel h, ← contract_contract]
   apply relRank_le_er
 
-@[simp] theorem relRank_empty_right (M : Matroid α) (X : Set α) : M.relRank X ∅ = 0 := by
+@[simp] lemma relRank_empty_right (M : Matroid α) (X : Set α) : M.relRank X ∅ = 0 := by
   rw [relRank_eq_er_contract, er_empty]
 
-@[simp] theorem relRank_empty_left (M : Matroid α) (X : Set α) : M.relRank ∅ X = M.er X := by
+@[simp] lemma relRank_empty_left (M : Matroid α) (X : Set α) : M.relRank ∅ X = M.er X := by
   rw [relRank_eq_er_contract, contract_empty]
 
-theorem relRank_eq_zero_of_subset (M : Matroid α) (h : Y ⊆ X) : M.relRank X Y = 0 := by
+lemma relRank_eq_zero_of_subset (M : Matroid α) (h : Y ⊆ X) : M.relRank X Y = 0 := by
   rw [relRank_eq_diff_right, diff_eq_empty.2 h, relRank_empty_right]
 
-@[simp] theorem relRank_cl_left (M : Matroid α) (X Y : Set α) :
+@[simp] lemma relRank_cl_left (M : Matroid α) (X Y : Set α) :
     M.relRank (M.cl X) Y = M.relRank X Y := by
   rw [relRank, relRank, contract_cl_eq_contract_delete, delete_er_eq', LoopEquiv.er_eq_er]
   rw [loopEquiv_iff_union_eq_union, contract_loops_eq, diff_union_self]
 
-@[simp] theorem relRank_cl_right (M : Matroid α) (X Y : Set α) :
+@[simp] lemma relRank_cl_right (M : Matroid α) (X Y : Set α) :
     M.relRank X (M.cl Y) = M.relRank X Y := by
   refine le_antisymm ?_ ?_
   · rw [relRank_eq_er_diff_contract,  relRank, ← (M ／ X).er_cl_eq Y, contract_cl_eq]
@@ -85,22 +85,22 @@ theorem relRank_eq_zero_of_subset (M : Matroid α) (h : Y ⊆ X) : M.relRank X Y
   exact er_mono _ <| (diff_subset _ _).trans
     ((M.subset_cl _).trans (M.cl_subset_cl (inter_subset_left _ _)))
 
-@[simp] theorem relRank_inter_ground_left (M : Matroid α) (X Y : Set α) :
+@[simp] lemma relRank_inter_ground_left (M : Matroid α) (X Y : Set α) :
     M.relRank (X ∩ M.E) Y = M.relRank X Y := by
   rw [←relRank_cl_left, cl_inter_ground, relRank_cl_left]
 
-@[simp] theorem relRank_inter_ground_right (M : Matroid α) (X Y : Set α) :
+@[simp] lemma relRank_inter_ground_right (M : Matroid α) (X Y : Set α) :
     M.relRank X (Y ∩ M.E) = M.relRank X Y := by
   rw [← relRank_cl_right, eq_comm, ← relRank_cl_right, cl_inter_ground]
 
-@[simp] theorem relRank_ground_left (M : Matroid α) (X : Set α) : M.relRank M.E X = 0 := by
+@[simp] lemma relRank_ground_left (M : Matroid α) (X : Set α) : M.relRank M.E X = 0 := by
   rw [← relRank_inter_ground_right, M.relRank_eq_zero_of_subset (inter_subset_right _ _)]
 
-theorem relRank_eq_relRank_union (M : Matroid α) (X Y : Set α) :
+lemma relRank_eq_relRank_union (M : Matroid α) (X Y : Set α) :
     M.relRank X Y = M.relRank X (Y ∪ X) := by
   rw [relRank, ← er_cl_eq, contract_cl_eq, ← relRank_eq_er_diff_contract, relRank_cl_right]
 
-theorem Basis'.relRank_eq_encard_diff (hI : M.Basis' I (X ∪ C)) (hIC : M.Basis' (I ∩ C) C) :
+lemma Basis'.relRank_eq_encard_diff (hI : M.Basis' I (X ∪ C)) (hIC : M.Basis' (I ∩ C) C) :
     M.relRank C X = (I \ C).encard := by
   rw [relRank_eq_relRank_union, relRank, ← er_cl_eq, contract_cl_eq, union_assoc, union_self,
     ← hI.cl_eq_cl, ← relRank_eq_er_diff_contract, relRank_cl_right,
@@ -110,30 +110,30 @@ theorem Basis'.relRank_eq_encard_diff (hI : M.Basis' I (X ∪ C)) (hIC : M.Basis
     union_eq_self_of_subset_left (inter_subset_right _ _)]
   exact disjoint_sdiff_left
 
-theorem Basis.relRank_eq_encard_diff (hI : M.Basis I (X ∪ C)) (hIC : M.Basis (I ∩ C) C) :
+lemma Basis.relRank_eq_encard_diff (hI : M.Basis I (X ∪ C)) (hIC : M.Basis (I ∩ C) C) :
     M.relRank C X = (I \ C).encard :=
   hI.basis'.relRank_eq_encard_diff hIC.basis'
 
-theorem Basis'.relRank_eq_encard_diff_of_subset (hI : M.Basis' I X) (hCX : C ⊆ X)
+lemma Basis'.relRank_eq_encard_diff_of_subset (hI : M.Basis' I X) (hCX : C ⊆ X)
     (hIC : M.Basis' (I ∩ C) C) : M.relRank C X = (I \ C).encard := by
   rw [← union_eq_self_of_subset_right hCX] at hI
   exact hI.relRank_eq_encard_diff hIC
 
-theorem Basis.relRank_eq_encard_diff_of_subset (hI : M.Basis I X) (hCX : C ⊆ X)
+lemma Basis.relRank_eq_encard_diff_of_subset (hI : M.Basis I X) (hCX : C ⊆ X)
     (hIC : M.Basis (I ∩ C) C) : M.relRank C X = (I \ C).encard :=
   hI.basis'.relRank_eq_encard_diff_of_subset hCX hIC.basis'
 
-theorem Indep.relRank_of_subset (hI : M.Indep I) (hJ : J ⊆ I) : M.relRank J I = (I \ J).encard := by
+lemma Indep.relRank_of_subset (hI : M.Indep I) (hJ : J ⊆ I) : M.relRank J I = (I \ J).encard := by
   rw [hI.basis_self.relRank_eq_encard_diff_of_subset hJ]
   rw [inter_eq_self_of_subset_right hJ]
   exact (hI.subset hJ).basis_self
 
-theorem Basis.relRank_eq_encard_diff_of_subset_basis (hI : M.Basis I X) (hJ : M.Basis J Y)
+lemma Basis.relRank_eq_encard_diff_of_subset_basis (hI : M.Basis I X) (hJ : M.Basis J Y)
     (hIJ : I ⊆ J) : M.relRank X Y = (J \ I).encard := by
   rw [← relRank_cl_left, ← hI.cl_eq_cl, relRank_cl_left, ← relRank_cl_right, ← hJ.cl_eq_cl,
     relRank_cl_right, hJ.indep.relRank_of_subset hIJ]
 
-theorem relRank_add_er_eq (M : Matroid α) (C X : Set α) :
+lemma relRank_add_er_eq (M : Matroid α) (C X : Set α) :
     M.relRank C X + M.er C = M.er (X ∪ C) := by
   obtain ⟨I, D, hIC, hD, -, hM⟩ := M.exists_eq_contract_indep_delete C
   obtain ⟨J, hJ, rfl⟩ :=
@@ -143,24 +143,28 @@ theorem relRank_add_er_eq (M : Matroid α) (C X : Set α) :
     ← hIC.encard, encard_diff_add_encard_inter, hJ.encard, ← union_inter_distrib_right,
     er_inter_ground_eq]
 
-theorem rFin.relRank_eq_sub (hY : M.rFin X) (hXY : X ⊆ Y) :
+lemma relRank_add_er_of_subset (M : Matroid α) (hXY : X ⊆ Y) :
+    M.relRank X Y + M.er X = M.er Y := by
+  rw [relRank_add_er_eq, union_eq_self_of_subset_right hXY]
+
+lemma rFin.relRank_eq_sub (hY : M.rFin X) (hXY : X ⊆ Y) :
     M.relRank X Y = M.er Y - M.er X := by
-  rw [← union_eq_self_of_subset_right hXY, ←relRank_add_er_eq, ← relRank_eq_relRank_union]
+  rw [← relRank_add_er_of_subset _ hXY]
   apply WithTop.add_right_cancel <| ne_top_of_lt hY
   rw [eq_comm, tsub_add_cancel_iff_le]
   exact le_add_self
 
-theorem Nonloop.relRank_add_one_eq (he : M.Nonloop e) (X : Set α) :
+lemma Nonloop.relRank_add_one_eq (he : M.Nonloop e) (X : Set α) :
     M.relRank {e} X + 1 = M.er (insert e X) := by
   rw [← union_singleton, ← relRank_add_er_eq, he.er_eq]
 
-theorem Nonloop.relRank_eq_sub_one (he : M.Nonloop e) (X : Set α) :
+lemma Nonloop.relRank_eq_sub_one (he : M.Nonloop e) (X : Set α) :
     M.relRank {e} X = M.er (insert e X) - 1 := by
   apply WithTop.add_right_cancel (show (1 : ℕ∞) ≠ ⊤ from ENat.coe_toNat_eq_self.mp rfl)
   rw [← he.relRank_add_one_eq, eq_comm, tsub_add_cancel_iff_le]
   exact le_add_self
 
-theorem relRank_add_of_subset_of_subset (M : Matroid α) (hXY : X ⊆ Y) (hYZ : Y ⊆ Z) :
+lemma relRank_add_of_subset_of_subset (M : Matroid α) (hXY : X ⊆ Y) (hYZ : Y ⊆ Z) :
     M.relRank X Y + M.relRank Y Z = M.relRank X Z := by
   obtain ⟨I, hI⟩ := M.exists_basis' X
   obtain ⟨J, hJ, hIJ⟩ := hI.indep.subset_basis'_of_subset (hI.subset.trans hXY)
@@ -176,17 +180,17 @@ theorem relRank_add_of_subset_of_subset (M : Matroid α) (hXY : X ⊆ Y) (hYZ : 
   exact disjoint_of_subset_left ((diff_subset _ _).trans (inter_subset_right _ _))
     disjoint_sdiff_right
 
-theorem relRank_eq_zero_iff (hY : Y ⊆ M.E := by aesop_mat) :
+lemma relRank_eq_zero_iff (hY : Y ⊆ M.E := by aesop_mat) :
     M.relRank X Y = 0 ↔ Y ⊆ M.cl X := by
   rw [← relRank_cl_left, relRank, er_eq_zero_iff', contract_loops_eq, cl_cl, diff_self,
     subset_empty_iff, contract_ground, ← inter_diff_assoc, inter_eq_self_of_subset_left hY,
     diff_eq_empty]
 
-theorem relRank_eq_zero_iff' : M.relRank X Y = 0 ↔ Y ∩ M.E ⊆ M.cl X := by
+lemma relRank_eq_zero_iff' : M.relRank X Y = 0 ↔ Y ∩ M.E ⊆ M.cl X := by
   rw [← relRank_inter_ground_right, ← relRank_inter_ground_left, relRank_eq_zero_iff,
     cl_inter_ground]
 
-theorem relRank_eq_one_iff (hY : Y ⊆ M.E := by aesop_mat) :
+lemma relRank_eq_one_iff (hY : Y ⊆ M.E := by aesop_mat) :
     M.relRank X Y = 1 ↔ ∃ e ∈ Y \ M.cl X, Y ⊆ M.cl (insert e X) := by
   rw [← relRank_cl_left, relRank_eq_er_diff_contract, er_eq_one_iff
     (show Y \ (M.cl X) ⊆ (M ／ (M.cl X)).E from diff_subset_diff_left hY)]
@@ -195,7 +199,7 @@ theorem relRank_eq_one_iff (hY : Y ⊆ M.E := by aesop_mat) :
     union_eq_self_of_subset_left (M.cl_subset_cl (subset_insert _ X))]
   exact ⟨fun ⟨e,he,_,hY'⟩ ↦ ⟨e,he,hY'⟩, fun ⟨e, he, hY'⟩ ↦ ⟨e, he, ⟨hY he.1, he.2⟩, hY'⟩⟩
 
-theorem relRank_le_one_iff (hYne : Y.Nonempty) (hY : Y ⊆ M.E := by aesop_mat) :
+lemma relRank_le_one_iff (hYne : Y.Nonempty) (hY : Y ⊆ M.E := by aesop_mat) :
     M.relRank X Y ≤ 1 ↔ ∃ e ∈ Y, Y ⊆ M.cl (insert e X) := by
   rw [le_iff_eq_or_lt, lt_iff_not_le, ENat.one_le_iff_ne_zero, not_not, relRank_eq_one_iff,
     relRank_eq_zero_iff]
@@ -209,20 +213,20 @@ theorem relRank_le_one_iff (hYne : Y.Nonempty) (hY : Y ⊆ M.E := by aesop_mat) 
   exact Or.inl ⟨_, ⟨hY'.1, he⟩, hY'.2⟩
 section Contract
 
-theorem er_contract_le_er (M : Matroid α) (C X : Set α) : (M ／ C).er X ≤ M.er X :=
+lemma er_contract_le_er (M : Matroid α) (C X : Set α) : (M ／ C).er X ≤ M.er X :=
   by
   obtain ⟨I, hI⟩ := (M ／ C).exists_basis (X ∩ (M ／ C).E)
   rw [← er_inter_ground_eq, ← hI.encard, ← hI.indep.of_contract.er]
   exact M.er_mono (hI.subset.trans (inter_subset_left _ _))
 
-theorem rFin.contract_rFin (h : M.rFin X) (C : Set α) : (M ／ C).rFin X := by
+lemma rFin.contract_rFin (h : M.rFin X) (C : Set α) : (M ／ C).rFin X := by
   rw [← er_lt_top_iff] at *; exact (er_contract_le_er _ _ _).trans_lt h
 
 lemma rFin.contract_rFin_of_subset_union (h : M.rFin Z) (X C : Set α) (hX : X ⊆ M.cl (Z ∪ C)) :
     (M ／ C).rFin (X \ C) :=
   (h.contract_rFin C).to_cl.subset (by rw [contract_cl_eq]; exact diff_subset_diff_left hX)
 
-theorem Minor.erk_le (h : N ≤m M) : N.erk ≤ M.erk := by
+lemma Minor.erk_le (h : N ≤m M) : N.erk ≤ M.erk := by
   obtain ⟨C, D, -, -, -, rfl⟩ := h
   rw [← er_univ_eq, ← er_univ_eq, delete_er_eq']
   exact (M.er_contract_le_er _ _).trans (M.er_mono (diff_subset _ _))
